RelationalAlgebra/Equivalence/RAtoFOL/Defs.lean
@@ -19,15 +19,11 @@ theorem ra_to_fol_query_schema [FOL.folStruc] (raQ : RA.Query) (dbs : DatabaseSc
     induction raQ
     all_goals simp_all [FOL.BoundedQuery.schema, ra_to_fol_query]
     case R rn =>
-      simp_all only [FOL.BoundedQuery.attributesInQuery, FOL.BoundedQuery.toFormula,
-        FirstOrder.Language.Relations.boundedFormula,
-        FirstOrder.Language.BoundedFormula.freeVarFinset, Function.comp_apply, FOL.outVar,
-        FirstOrder.Language.Term.varFinsetLeft.eq_1]
       ext a
-      simp_all only [Finset.mem_biUnion, Finset.mem_univ, Finset.mem_singleton, true_and]
+      simp_all only [FOL.outVar, FirstOrder.Language.Term.varFinsetLeft, Finset.mem_singleton,
+        Set.mem_toFinset, Set.mem_setOf_eq]
       apply Iff.intro
-      · intro a_1
-        obtain ⟨w, h⟩ := a_1
+      · intro ⟨w, h⟩
         subst h
         exact RelationSchema.fromIndex_mem w
       · intro a_1
@@ -43,20 +39,15 @@ theorem ra_to_fol_query.isWellTyped [FOL.folStruc] (raQ : RA.Query) (dbs : Datab
     case R dbs rn => exact h
 
     case s q a b pos sq ih =>
-      simp_all only [RA.Query.isWellTyped, ← ra_to_fol_query_schema, ne_eq, ra_to_fol_query,
-        FOL.outVar, FOL.BoundedQuery.isWellTyped.tEq_def, FirstOrder.Language.Term.varFinsetLeft,
-        FOL.BoundedQuery.isWellTyped.schema_eq_attributesInQuery,
-        FOL.BoundedQuery.attributesInQuery, Finset.union_subset_iff, Finset.singleton_subset_iff,
-        true_and, forall_const, and_self]
+      simp_all [RA.Query.isWellTyped, ← ra_to_fol_query_schema, ra_to_fol_query,
+        FOL.outVar, Finset.union_subset_iff]
 
     case p rs sq ih =>
       simp_all only [RA.Query.isWellTyped, ← ra_to_fol_query_schema, ra_to_fol_query,
-        projectQuery, FOL.BoundedQuery.attributesInQuery, Nat.add_zero,
-        FOL.BoundedQuery.isWellTyped.exs_def, FOL.BoundedQuery.relabel_isWellTyped]
+        projectQuery, FOL.BoundedQuery.isWellTyped.exs_def, FOL.BoundedQuery.relabel_isWellTyped]
 
     case j q₁ q₂ q₁_ih q₂_ih =>
-      simp_all only [RA.Query.isWellTyped, ra_to_fol_query,
-        FOL.BoundedQuery.isWellTyped.and_def, and_self]
+      simp_all [RA.Query.isWellTyped, ra_to_fol_query,]
 
     case r f q q_ih =>
       simp_all only [RA.Query.isWellTyped, ra_to_fol_query,
